Generalize Pi to TBind so we have both sigma and pi

syntax.sig
@@ -1,13 +1,16 @@
 nat  : Type
 Tm(VarTm) : Type
 PTag : Type
+TTag : Type
 
+TPi : TTag
+TSig : TTag
 PL : PTag
 PR : PTag
 Abs : (bind Tm in Tm) -> Tm
 App : Tm -> Tm -> Tm
 Pair : Tm -> Tm -> Tm
 Proj : PTag -> Tm -> Tm
-Pi : Tm -> (bind Tm in Tm) -> Tm
+TBind : TTag -> Tm -> (bind Tm in Tm) -> Tm
 Bot : Tm
 Univ : nat -> Tm
